src/equiv/PtoPF.v
@@ -53,9 +53,9 @@ Proof.
                          lc0.(Local.vwo)
                          lc0.(Local.vcap)
                          lc0.(Local.vrel)
-                         lc0.(Local.vpn)
-                         lc0.(Local.lper)
-                         lc0.(Local.per)
+                         lc0.(Local.vpr)
+                         lc0.(Local.vpa)
+                         lc0.(Local.vpc)
                          lc0.(Local.fwdbank)
                          lc0.(Local.exbank)
                          (Promises.set (S (length mem1)) lc0.(Local.promises))).
